# **Lecture 37 — Martingales for Brownian Motion**
STT 882  
April 21, 2025

## 1. Martingales in Continuous Time

Consider a filtered probability space  
$$(\Omega,\mathcal F, \{\mathcal F_t\}_{t\ge 0}, P).$$

A process $\{X_t,\mathcal F_t\}_{t\ge 0}$ is a **martingale** if:

1. $E|X_t| < \infty$ for all $t \ge 0$.
2. $X_t$ is $\mathcal F_t$-measurable.
3. $E[X_{t+h} \mid \mathcal F_t] = X_t$ for all $t\ge0$, $h>0$.

We want to study martingales **associated with Brownian motion**, using its natural (canonical) filtration $\{\mathcal F_t\}$.

Let
$$
M:\mathbb R \times [0,\infty) \to \mathbb R,\qquad (x,t)\mapsto M(x,t).
$$

**Main question:**  
When is the process  
$$
M(B_t^x, t),\qquad t\ge0,
$$
a martingale?

This requires
$$
E_x\!\left[\,M(B_{t+h}, t+h)\mid \mathcal F_t \right]
   = M(B_t, t)
   \quad\text{a.s. for all } x\in\mathbb R,\ t\ge 0,\ h>0.
$$

By the Markov property of Brownian motion,
$$
E_x[M(B_{t+h},t+h)\mid \mathcal F_t]
    = E_{B_t}[M(B_h,t+h)].
$$

Define
$$
\varphi(y)=E_y[M(B_h,t+h)].
$$
The condition becomes
$$
\varphi(B_t)= M(B_t,t).
$$

---

## 2. Example: The Famous Exponential Martingale

Define, for $\theta\in\mathbb R$,
$$
M(x,t)=\exp(\theta x - \tfrac12\theta^2 t).
$$

Then, with $B_{t+h}\sim N(x,h)$,
$$
\begin{aligned}
E_x[M(B_{t+h},t+h)]
 &= E_x\left[\exp\left(\theta B_{t+h}-\frac12\theta^2(t+h)\right)\right] \\
 &= e^{-\frac12\theta^2(t+h)} E_x(e^{\theta B_{t+h}}).
\end{aligned}
$$

Write
$$
B_{t+h}=x+\sqrt{h}Z,\qquad Z\sim N(0,1).
$$

Then
$$
\begin{aligned}
E_x(e^{\theta B_{t+h}})
 &= e^{\theta x} E(e^{\theta\sqrt h\, Z})
  = e^{\theta x} e^{\frac12 \theta^2 h}.
\end{aligned}
$$

Putting it together,
$$
E_x[M(B_{t+h},t+h)]
  = e^{-\frac12\theta^2 t} e^{\theta x}
  = M(x,t).
$$

Thus the process
$$
\boxed{\,e^{\theta B_t - \frac12\theta^2 t}\,}
$$
is a martingale under $P_x$ for every $x\in\mathbb R$.

---

## 3. Differentiating the Exponential Martingale

Because
$$
E_x\Big[ M(B_{t+h},t+h;\theta)\Big] = M(x,t;\theta)
$$
for all $\theta$, we may differentiate under the expectation.

### First derivative w.r.t. $\theta$:

$$
\frac{\partial}{\partial\theta}M(x,t;\theta)
   = (x-\theta t)\, M(x,t;\theta).
$$

Evaluate at $\theta=0$:
$$
\left.\frac{\partial}{\partial\theta}M(x,t;\theta)\right|_{\theta=0}
 = x.
$$

Thus the process
$$
\boxed{\,B_t\,}
$$
is a martingale.

### Second derivative:

$$
\frac{\partial^2}{\partial\theta^2} M(x,t;\theta)
 = (x-\theta t)^2 M(x,t;\theta).
$$

Evaluate at $\theta=0$:
$$
\left.\frac{\partial^2}{\partial\theta^2}M(x,t;\theta)\right|_{\theta=0}
 = x^2.
$$

Thus
$$
\boxed{\,B_t^2 - t\,}
$$
is a martingale.

### Third derivative:

Written out (from notes on page 3),
$$
\frac{\partial^3}{\partial\theta^3}M
= M(\cdot)(x-\theta t)^3 + M(\cdot)\cdot 2(x-\theta t)(-t)
     -tM(\cdot)(x-\theta t).
$$

At $\theta=0$, this produces the martingale
$$
\boxed{\,B_t^3 - 3t B_t\,}.
$$

Continuing similarly gives the whole **Hermite–polynomial martingale family**:
$$
1,\quad
B_t,\quad
B_t^2 - t,\quad
B_t^3 - 3 t B_t,\quad
B_t^4 - 6 t B_t^2 + 3t^2,\ \ldots
$$

---

## 4. PDE Characterization of Martingales

A smooth function $M(x,t)$ satisfies
$$
\boxed{\qquad
\frac{\partial M}{\partial t}
+ \frac12 \frac{\partial^2 M}{\partial x^2} = 0,
\qquad x\in\mathbb R,\ t>0,
}
$$
if and only if
$$
M(B_t,t)
$$
is a martingale.

This is the **backward heat equation**.

The book proves:
$$
\frac{d}{dt} E_x[M(B_t,t)] = 0,
$$
so
$$
\boxed{\quad E_x[M(B_t,t)] = M(x,0),\quad t\ge 0.\quad}
$$

---

## 5. Connection with Brownian Transition Density

The transition density of Brownian motion is
$$
P_t(x,y)
   = \frac{1}{\sqrt{2\pi t}}
      \exp\!\left(-\frac{(y-x)^2}{2t}\right)
   = p_{N(x,t)}(y).
$$

It satisfies the forward heat equation:
$$
\frac{\partial P_t}{\partial t}
   = \frac12 \frac{\partial^2 P_t}{\partial y^2}.
$$

This PDE duality explains why solving the backward heat equation produces martingales.

---

## 6. Optional Stopping for These Martingales

For a stopping time $\tau$ with $\tau \le t$ a.s., the optional stopping theorem gives
$$
E_x\!\left[M(B_t,t)\mid\mathcal F_\tau\right]
   = M(B_\tau,\tau).
$$

This holds for all martingales $M(B_t,t)$ generated by the backward heat equation.

---

# **End of Lecture 38**
