we wart is Extend to step 3.
setup: $f \geq 0, \mu$ - is $\sigma$-finite.
$(\Omega, F, M), f \in F\left(f: \Omega \rightarrow \mathbb{R}\right.$ is Bonel Measureate" i.e. $f^{-1}(B) \in F$, $\forall B$-Brel subset

$$
\begin{aligned}
& \delta_{\Omega} f \delta \mu=I(f) \\
& \int_{E} f \partial \mu=\left.I(f)\right|_{\Omega} \left\lvert\, \begin{array}{l}
I(f) \equiv \sup \{I(h): f \geq h \geq 0, h \text { bad, } \mu(x: h(x)>0)<\infty\} \\
\bigcup_{n=1}^{E_{n+1}} E_{n}=\Omega
\end{array}\right.
\end{aligned}
$$

Lemma ${ }_{\text {min. }}$ Let $E_{n} \uparrow \Omega, E_{n} \in F, \mu\left(E_{n}\right)<\infty, n \geq 1$ then

$$
I\left(f \stackrel{\text { min. }}{\text { seq. of }} \cap j E_{n}\right) \uparrow I(f)
$$

$$
\lim _{n \rightarrow \infty} I\left(f \wedge \cap j E_{n}\right) \underset{n \rightarrow \infty}{\rightarrow} I\left[\lim _{n \rightarrow \infty}\left[(f \wedge n) \cdot \mathbb{1}_{E_{n}}\right]=I(f)\right.
$$

curswitch Between Lum 3 Int. sometimes con't switch.

## Monotone convergence theory.

if $f_{n} \geq 0, f_{n} \uparrow f$ as $n \rightarrow \infty$ (almost everywhere a.e. then

Does not mean
$\forall \omega \in \Omega: f_{n}(\omega) \uparrow f(\omega)$
$\mu\left(f_{n} \uparrow f\right)=0$
Mexsures of zero Don't go into Integral so Ig arove.

Don't od
Prove: N.T.S. $\forall h . \geq 0$, bounded, $\mu(h>0)<\infty$
$\lim _{n \rightarrow \infty} I\left(F \wedge_{n, j} E_{n}\right) \geq I(h)$.
obviously smaller then $f$
Assume: $0 \leq G^{\text {By Bounded. }}$

$$
\begin{aligned}
\Rightarrow \forall n \geq & \begin{array}{l}
M \text { upeget } 0 \leq h \leq f \wedge_{n} \\
\text { becaule of ADPitivitg. }
\end{array} \\
I(h)= & I\left(h_{j} E_{n}\right)+I\left(h j E_{n}^{c}\right) \\
& \int_{\Omega} h \wedge E_{n} \delta u+\int_{\Omega} h^{\wedge} E_{n}^{c} \partial u
\end{aligned}
$$

$$
\begin{aligned}
& \partial_{\Omega}^{h \wedge E_{n} \partial u}+\int_{\Omega} h^{\wedge} E_{n}^{-} \partial u \\
\leq & I\left(f \wedge \cap ; E_{n}\right)+M \cdot \mu\left(E_{n}^{c} \cap\{h>0\}\right)^{2000} \text { (adtl. hot. } \\
& E_{n}^{c} \cap\{\omega: h(\omega)>0\} . \\
& E_{n}^{c} \downarrow \phi
\end{aligned}
$$

$B_{n}$
$\bigcap_{n \in E^{\prime}}^{\infty} E_{n}^{c}=\phi$
NTS M $\mu(\overbrace{E_{n}^{c} \cap\left\{h>0^{2}\right\}}) \rightarrow 0$
$E_{n} \supset E_{n+1}^{c} \subset \cap \geq 1$
we have: $B_{n} \nrightarrow \phi, \mu\left(B_{1}\right)<\infty \quad \mu\left(B_{n}\right) \nmid 0$
Cumpact means cloces and oper Bounded.
Dissoint
$B_{1}=\bigcup_{k=1}^{\infty} B_{k} \backslash B_{k+1} \cup \bigcap_{k=1}^{\infty} B_{k} \begin{gathered}K_{k} \\ \text { means this } \phi\end{gathered}$
This is not true.

$$
\mu\left(B_{1}\right)=\sum_{k=1}^{\infty}\left[\mu\left(B_{k}\right)-\mu\left(B_{k+1}\right)\right]
$$

![](https://cdn.mathpix.com/cropped/2025_11_26_4bb208c2eae9bb28e36fg-2.jpg?height=315&width=374&top_left_y=938&top_left_x=1359)
if $\sum_{k=1}^{\infty} \mu\left(B_{k}\right)-\mu\left(B_{k+1}\right)$ tele scoping some sots.

$$
\begin{aligned}
& =\mu\left(B_{1}\right)-\mu\left(B_{n}+1\right) \xrightarrow{n \rightarrow \infty} \mu\left(B_{2}\right) \\
& =\mu\left(B_{n+1}\right) \xrightarrow[n \rightarrow \infty]{ } 0
\end{aligned}
$$

![](https://cdn.mathpix.com/cropped/2025_11_26_4bb208c2eae9bb28e36fg-2.jpg?height=353&width=436&top_left_y=1411&top_left_x=1387)
Proof: Finest Directan.

can use hashithe But meabe more his

$$
\begin{aligned}
& \text { can ree hashithe if so sup is Biggres. } \\
& I(f)+I(g)=\operatorname{Sup}_{\substack{0<h_{1} \leqslant f \\
0 \leqslant h}} I\left(h_{1}+h_{2}\right) \leq \operatorname{Sup}_{0 \leqslant h \leqslant \text { fag }} I(h)^{\prime * \text { so }}=I(8+2) \\
& 0 \leq h_{2} \leq g \\
& \begin{array}{l}
h \quad b d a \\
\mu(h>0)<\infty
\end{array} \\
& M\left(h_{i}>0\right)<\infty \\
& \mu\left(m_{2}>0\right)<\infty \\
& \text { his he Bad. }
\end{aligned}
$$

$$
(A+g) \wedge n \leq(f \wedge n)+(g \wedge n)
$$

$$
I\left((E+g) \wedge n ; E_{n}\right)
$$

Care.1: $f>n$ or $g>n$
cuse 7: $g<n$ and $g<n$
$I$ ( $\left(E+g \lambda \wedge n j E_{n}\right)$
![](https://cdn.mathpix.com/cropped/2025_11_26_4bb208c2eae9bb28e36fg-3.jpg?height=319&width=1390&top_left_y=195&top_left_x=243)

Define $I(f)$ when $I(|f|)<\infty$

$$
f=f^{+}-f^{-} \quad f^{+}=f \vee 0 \underset{\text { positive }}{f^{-}}=(f \wedge 0)(-1)
$$

we knows how to integate Euch..

$$
\begin{aligned}
& \quad|f|=f^{+}+f^{-} \Rightarrow \quad I\left(\delta^{+}\right)<\infty \\
& I(f)=I\left(f^{+}\right)-I\left(f^{-}\right)
\end{aligned}
$$

Proving ADDitivity Ror fig with $I(|S|)<\infty, I(|g|)<\infty$ when $I(|f|)<\infty \rightarrow$ is integrable.
if $\rho>0$ Then $I(f)$ is Alwen defined. (We cer have $I(P)=\infty$,)

$$
\begin{array}{rl}
I(\rho+g) & =I\left(f^{+}-\rho^{-}+g^{+}-g^{-1}\right) \\
& =I\left(f^{+}+g^{+}-\left(f^{2}+g^{-1}\right)\right)-\text { use ADD-1ing Becuuse All protipe } \\
& =I\left(f^{+}+g^{+}\right)-\left(I\left(f^{-}\right)+I\left(g^{-1}\right)\right) \\
& =I(f)+I(g) \\
f, g \geq 0 & I(F-2)=I(f)-I(g)
\end{array}
$$

