(1) Def: $x_{n} \Rightarrow x$ if $P\left(x_{n} \leq x\right) \xrightarrow{n \rightarrow \infty} P(x \leq x), \forall x$ s.t. $P\left(\frac{\underset{0}{\Pi}}{\text { II }}=x\right)=0$
.Def (2) $\underline{X}_{n} \Rightarrow \underline{Z}$ if $E g\left(X_{n}\right) \xrightarrow[n \rightarrow 00]{ } E g(\underline{z}), g \in C_{B}(\mathbb{R}) \quad F_{x}(x-)=F_{\underline{Z}}(x)$
![](https://cdn.mathpix.com/cropped/2025_11_26_29a83eb473355dea954fg-1.jpg?height=203&width=1699&top_left_y=397&top_left_x=143)
theorem A if $X_{n} \Rightarrow X$ then, $\exists(\Omega, \mathcal{Z}, P)$ and P.V.S $Y_{n}$, $Y$ s.t.
$Y_{n} \stackrel{D}{=} X_{n}, n>1, \quad Y \stackrel{D}{=} x$ and. $Y_{n} \stackrel{\text { as }}{\overrightarrow{n \rightarrow \infty}} Y$
then to gos from $\operatorname{DeF}$ (1) is $\operatorname{Def}$ (2) use theoren $A$

Assume (i), we use the theores
"this in Errough"

$$
E g\left(v_{n}\right) \xrightarrow[n \rightarrow \infty]{ } E g(v)
$$

$Y_{n} \xrightarrow[n \rightarrow \infty]{\text { a.s. } Y}$ so we conclude that $g\left(Y_{n}\right) \xrightarrow[a \cdot s_{s}]{\text { By Continutly. }} g(Y)$
by DCT $E g\left(y_{0}\right) \xrightarrow[n \rightarrow \infty]{ } E(g(y))$

$$
|g(x)| \leqslant c<\infty, \quad x \in \mathbb{R} .
$$

we get (2)
Let $Y$ be a c.v. and $F(y)=p(Y \leq y), y \in \mathbb{R}$
We need $F^{-1}(p), 0 \leq p \leq 1$

$$
F^{-1}(P)=\operatorname{Sup}\{y: F(y)<P\} \quad 0 \leq P \leq 1
$$

Step 1
Clasm let $U \sim$ vaiform $(0,1)$
three ases.
Nice case cof.
![](https://cdn.mathpix.com/cropped/2025_11_26_29a83eb473355dea954fg-1.jpg?height=214&width=412&top_left_y=1409&top_left_x=1241)

Jenp case
![](https://cdn.mathpix.com/cropped/2025_11_26_29a83eb473355dea954fg-1.jpg?height=196&width=394&top_left_y=1654&top_left_x=1248)

$$
\begin{array}{ll}
F^{-1}(W) \stackrel{\infty}{=} Y^{\text {Result. }} & P(0 \leq x)=x, 0 \leq x \leq 1 \\
P\left(F^{-1}(u)<y\right)=P(u<F(y))=F(y)=p(y \leq y), y \in \mathbb{R}
\end{array}
$$

![](https://cdn.mathpix.com/cropped/2025_11_26_29a83eb473355dea954fg-1.jpg?height=233&width=396&top_left_y=1811&top_left_x=1239)
step2 if $F_{n}^{f}(y) \xrightarrow[n \rightarrow \infty]{\rightarrow \infty} F(y), F(y)>F(y-)$
then $F_{n}^{-1}(u) \underset{n \rightarrow \infty}{\rightarrow} F^{-1}(u), \quad 0<u<1$
$F_{n}^{-1}(u)$
$U \sim$ uniform 0,1 ): $F_{n}^{-1}(W) \xrightarrow[n \rightarrow \infty]{\text { a.s. }} F^{-1}(W)$
![](https://cdn.mathpix.com/cropped/2025_11_26_29a83eb473355dea954fg-1.jpg?height=248&width=194&top_left_y=2101&top_left_x=1293)

$$
Y_{n} \xrightarrow[n \rightarrow \infty]{\text { as }} Y^{\| \mathcal{D}}
$$

Proof from ${ }^{\text {pef }}(2)$ To (1)
take $x \in \mathbb{R}$ s.t. $F_{\bar{x}}(x)=F_{\bar{x}}(x-) \quad(P(z=x)=0)$
![](https://cdn.mathpix.com/cropped/2025_11_26_29a83eb473355dea954fg-2.jpg?height=229&width=410&top_left_y=228&top_left_x=281)

$$
\begin{aligned}
& P\left(\bar{z}_{n} \sim x\right) \leqq \int_{0}^{x+\epsilon} g_{x, \varepsilon}(y) \delta F_{z_{n}}(y) \\
& \text { Note } \\
& 1=\int_{\partial}^{+} g_{x, \varepsilon}(y) \partial F_{x}(y) \\
& \lim _{n \rightarrow \infty} P\left(Z_{n} \leq x\right) \leq P(Z \leq x+2) \\
& P(Z \leq x+\varepsilon) \underset{\varepsilon \rightarrow 0}{\longrightarrow} P(x \leq x) \\
& P(x=x)=0 .
\end{aligned}
$$

we need $\lim _{n \rightarrow \infty} P\left(\underline{x}_{n} \geq x\right) \geq P(\underline{x}<x)$ i $P(x \leqslant x)$
Cirs $=\overline{\lim }$ the equality.
![](https://cdn.mathpix.com/cropped/2025_11_26_29a83eb473355dea954fg-2.jpg?height=235&width=384&top_left_y=1016&top_left_x=1422)

Both $g_{x, \varepsilon} g_{x,-\varepsilon}$ Are uniformly conthyous.
Continuith. $F$ is continuous at $x$
$\forall \varepsilon>0, \exists \delta<0$ s.ts $|f(x+0)-f(x)| \cdot<\varepsilon, \quad|u|<\delta(x)$
uniformly curtinuous neen use $A x y<\delta \neq \delta(x), x \in R$
Enough to chack $P^{E}(2)$ for I Bounded 3 uniformly cont.
Also hem infinite Derivather.
Suys
![](https://cdn.mathpix.com/cropped/2025_11_26_29a83eb473355dea954fg-2.jpg?height=159&width=392&top_left_y=1833&top_left_x=439)

Examples (1) $Z_{n} \equiv a_{n}{ }^{4 \text { costant }}, Z=a$
$Z_{n} \Rightarrow$ iff $a_{r} \underset{n \rightarrow \infty}{\rightarrow \infty} a$
(2) $X_{n} \xrightarrow[n \rightarrow \infty]{\text { a.s. }}$ then we have Also. $X_{n} \Rightarrow x$
(3) $Y_{n} \sim$ Geometric $\left(\frac{\lambda}{n}\right), n \geq 1$
$\frac{Y_{n}}{n} \Longrightarrow Y \sim \exp (\lambda)$
$Z \sim$ Geometric ( $p$ ), $0<p<1$

$$
\begin{aligned}
& P(z>k)=(1-P)^{k}, k=1,2 \ldots \\
& P\left(\frac{Y_{n}}{n}>t\right)=P\left(Y_{n}>n t\right)=\left[\left(1-\frac{\lambda}{n}\right)^{n}\right] \underset{n \rightarrow 0}{\longrightarrow} e^{-\lambda t}<P(y>t), t \geq 0
\end{aligned}
$$

Example 4
$\left\{z_{i}\right\}_{i \geq 1}$ iid $p\left(x_{i}=k\right)=\frac{1}{N}, k=1,2 \ldots, N$
First Tome there is a tire
$T_{N}=\min \left\{n \geq 2: \exists i<n\right.$ with $\left.S_{i}=x_{n}\right\}$.
$P\left(T_{N}>n\right)=\frac{N(n-1) \ldots(N-n-1)}{N^{n}}=\prod_{m=2}^{n}\left(1-\frac{m-1}{N}\right)$
$n>N$ tie for some
Cook at $x_{1}, \ldots x_{n}$
we Ane intereghed in $P\left(\frac{T_{N}}{\sqrt{n}}>y\right)=P\left(T_{n}>\sqrt{N} \cdot y\right)=\sum_{n=2}^{\sqrt{N K}}\left(1-\frac{M-1}{N}\right) \rightarrow_{N \rightarrow \infty}^{2+3+4 \ldots} e^{-\frac{y^{2}}{2}} P\left(\frac{T_{N}}{\sqrt{N}} \leq y\right) \underset{y \rightarrow 100}{\longrightarrow} 1-e^{-\frac{y^{2}}{z}} \quad y \geq b$

