$P\left(X_{n}=k\right) \underset{n \rightarrow \infty}{\longrightarrow} P(x=k), k \in \mathbb{Z}$
Tr.k $P_{k} \quad G$ Genuine Probabilies?
$\begin{array}{ll}N^{3} & \sum_{k \in \mathbb{Z}} P_{n_{k}}=1 \\ & \sum_{k \in Z} P_{k}=1 \\ P_{r}=\left(P_{n k} \geq 0\right)_{k \in Z} & P=\left(P_{k} \geq 0\right)_{k \in Z}\end{array}$
then $\left\|P_{n}-P\right\|=\sum_{k \in \mathbb{T}}\left(P_{n, k}-P_{, k}\right) \xrightarrow[n \rightarrow \infty]{ } 0$
$P\left(x_{n} \leq k\right)-P(x \leq k) \underset{n \rightarrow \infty}{\longrightarrow} 0, k \in \mathbb{Z}$
wts. $\left|\sum_{l \leq k} P_{n . l}-\sum_{l \leq k} P_{l}\right| \xrightarrow[n \rightarrow \infty]{ } 0 \quad k \in \mathbb{Z}$

$$
\begin{aligned}
& \left\|P_{n}-P\right\| \geq \sum_{l \leq k}^{11}\left|P_{n-l}-P_{l}\right| \underset{n=\infty}{\rightarrow} \\
& \left|P_{n, k}-P_{k}\right|=\left(P_{k}-P_{n, k}\right)^{+}+\left(P_{k}-P_{n, k}\right)^{-} \\
& P_{k}-P_{n, k}=\left(P_{k}-P_{n, k}\right)^{+}-\left(P_{k}-P_{n, k}\right)^{-} \\
& \sum_{k}\left(P_{k}-P_{n, k}\right)=\sum_{k}\left(P_{k}-P_{n, k}\right)^{k}-\sum_{k}\left(P_{k}-P_{n, k}\right)^{-} \\
& \sum_{k} P_{k}=1 \\
& \sum_{k} P_{i_{1 n}}=1 \\
& \sum_{k}\left|P_{n, k}-P_{k}\right|=\sum_{k}\left(P_{k}-P_{h_{1} k}\right)^{t}+\sum_{k}\left(P_{k}-P_{a_{1} k}\right)=2 \sum_{k} \sum\left(P_{k}-P_{n_{1} k}\right)^{t} \leq 2 \sum_{k}^{\quad / \quad \text { since } \quad P_{k} \quad P_{3} t} \\
& \therefore P_{n k} \xrightarrow[n]{ } P_{k}, k \in z .
\end{aligned}
$$

insest Dominace anverne theorem, DCt.
$f_{n}, f:(\Omega, \mathcal{F}, \mu) \rightarrow \mathbb{R}$.
$\mu-\sigma f$ nite necoure
$f_{n}, \forall:(\Omega, \mathcal{F}, \mu) \rightarrow \mathbb{K}$.
$\mu-\sigma$ finite measure

$$
\Omega_{n} C \Omega, \psi \Omega_{n}=\Omega, \mu\left(\Omega_{n}\right) \uparrow M(r)
$$

$M\left(\Omega_{n}\right)<\infty$
if $f_{n}(\omega) \xrightarrow[n \rightarrow \infty]{ } f(\omega)$, N-a.e.
and $\left|f_{n}(\omega)\right| \leq g(\omega)$ with $\int_{\Omega} g \delta \mu<\infty$
then $\int_{\Omega} F_{n} d r \rightarrow \int_{\Omega} F_{\theta} d x$
$\Omega=\mathbb{Z},\{\mathcal{F}$ all subsets of $\mathbb{Z}\}, \mu(k)=1, k \in \mathbb{K} M(A)=$ cordinalits of $A$.

$$
a=\left(a_{n}\right)_{n \in \mathbb{Z}}
$$

$+18$

$$
\int_{\Omega} a_{\partial \mu}=\sum_{n \in \mathbb{Z}} a_{n}
$$

$\forall k \in \mathbb{R}$.

$$
P_{\text {nik }} \underset{n \rightarrow \infty}{\longrightarrow} P_{k}
$$

$P_{K} \geq\left(P_{K}-P_{n \cdot K}\right)+\underset{K \rightarrow \infty}{\longrightarrow} 0$
then $\left\|P_{n}-P\right\|=\Sigma\left|P_{n, x}-P_{k}\right| \xrightarrow[n \rightarrow 0]{ } 0 \mathrm{~J}$ By DOT.

$$
f_{x_{n}}(x)-f_{n}(x), \quad f_{x}(x)=f_{n}(x),
$$

statenuit
if $f_{n}(x)_{n \rightarrow \infty} f(x)_{1} x \in \mathbb{R}$.
Then $\int_{x \in \mathbb{R}}\left|f_{n}(x)-f(x)\right| \partial x \underset{n \rightarrow \infty}{\rightarrow} 0$

$$
\left\|\mu_{\alpha_{n}}-\mu_{x}\right\| \underset{n \rightarrow \infty}{\rightarrow} 0
$$

$+2 k \hat{r}_{k=1}^{\wedge}\left(1+a_{a_{k}}\right) \xrightarrow[n \rightarrow \infty]{ } e^{c} \quad$ Triangle Arrig of Bermiblis.
$+2 k \hat{\eta}_{k=1}^{\hat{\eta}}\left(1+a_{n, k}\right) \xrightarrow[n \rightarrow \infty]{ } e^{c} \quad$ Triencile Arriez of Bervidilks.

$$
\sum_{k=1}^{n} a_{n k} \rightarrow_{n \rightarrow \infty} a
$$

Heorene if $\left\{X_{n, m}\right\}_{1 \leq m \leq n}, n>1,\left\{X_{n m}\right\}_{1 \leq m \leq n} \quad X_{n, m} \sim \operatorname{Ber}\left(P_{n, m}\right)$
if (1) $\sum_{m=1}^{n} P_{n i n} \xrightarrow[n \rightarrow \infty]{ } \lambda$
(2) Mut $P_{\text {nin }} \longrightarrow 0$
$1 \leq m \leq n$
there $S_{n}=\sum_{n=1}^{n} t_{n} m \Rightarrow$ Poisgon. "So we know it canceree in Total Uniterton.

+ $58^{\text {" }}$ we went a proff for commounse in unform."
Gool

$$
\begin{aligned}
& P_{n}=\left(P_{n, m}\right)_{1 s m \pm n, n \geq 1} \\
& P=\left(P_{m}\right)_{1 \leq m} \\
& \left\|P_{n}-P\right\|=\sum_{m=1}^{\infty}\left|P\left(x_{n}=m\right)-P(x=m)\right|
\end{aligned}
$$

instero.
we will look At total veriattas.

$$
\begin{aligned}
& Q_{n}=\left(q_{n i m}\right)_{1 \leq m} \\
& q_{n}=P\left(\operatorname{Poison}\left(\sum_{n=1}^{n} P_{n, m}\right)\right)
\end{aligned}
$$

Goal: $\left\|P_{n}-q_{n}\right\| \leq 2 \sum_{m=1}^{n} P_{n, m}^{2}$
![](https://cdn.mathpix.com/cropped/2025_11_26_bbc1444001dc06821efbg-3.jpg?height=101&width=1334&top_left_y=2119&top_left_x=221)

$$
\leqslant \eta \cdot\left(\frac{\lambda}{r}\right)^{2} \leq 2 \frac{\lambda \lambda^{2}}{\lambda}
$$

![](https://cdn.mathpix.com/cropped/2025_11_26_bbc1444001dc06821efbg-3.jpg?height=119&width=1101&top_left_y=2426&top_left_x=273)

Redefine

$$
q_{n}=P(\text { Poissool }
$$

$$
\begin{aligned}
& \left.\left\|\mu_{1} \times \mu_{2}-J_{1} \times J_{2}\right\| \leq\left\|\mu_{1}-J_{1}\right\|+\| \mu_{2}-J_{2}\right) \\
& \text { Step } 1 \\
& \mu_{L}=\text { zinst of } \alpha \\
& \text { MLL }=\partial \sin \text { of } K \\
& x \perp 4 . \\
& M_{1}>M_{2}(k, l)=P(x=1 A)(4 \times l) \\
& M_{1} \times M_{2}(k, l)-V_{1} \not y V_{2}(k, l) \\
& =\mu_{1}(l) \cdot \mu_{2}(l)-V_{1}(l) V_{2}(l) \\
& =\mu_{1}(l) \mu_{2}(l)-\mu_{1}(k) V_{2}(l)-\mu_{1}(k) V_{2}(l)-V_{1}(k) V_{2}(l) \mid \\
& \text { with } \sum_{e} \sum_{e} V_{2}(e) \backslash \\
& =\sum \underline{\mu_{1}(k)}=\mid M_{2}(l)-V_{2}(l)+V_{2}^{2} C M_{1}(k)-V_{1}(k) \cdot f \\
& \left.\varepsilon m_{1} k\right) \| m_{2}-v_{2} \quad \mid\left(m_{1}-v_{2} \|\right)
\end{aligned}
$$

$$
\| n_{2}-V_{n} \geqslant
$$

convelution
Step $2\left\|\mu_{1} * \mu_{2}-V_{1} * V_{2}\right\| \delta\left\|\mu_{1} \times \mu_{2}-V_{1} \times V_{2}\right\|$

$$
\mu_{1} * \mu_{n}(k)-P(x+\gamma-k)=\sum_{l} \mu_{1}(l) \mu_{2}(k-l)
$$

Bout to companing.

$$
\begin{aligned}
\left\|\mu_{1} * \mu_{2}-v_{1} * v_{2}\right\| & =\sum_{1} \sum_{l} \mu_{l}(l) \mu_{2}(k-l)-\sum_{k} \sum_{l} v_{1}(l) v_{2}(k-l) \\
& \leq \sum_{k} \sum_{l} \mu_{1}(l) \mu_{c}(k-l)-v_{1}(l) v_{2}(1-l) \\
& =\left\|\mu_{1} \times \mu_{2}-v_{11} \times \sigma_{2}\right\|
\end{aligned}
$$

![](https://cdn.mathpix.com/cropped/2025_11_26_bbc1444001dc06821efbg-4.jpg?height=396&width=355&top_left_y=1987&top_left_x=299)
"They is smear
anote: $\left\|\mu_{1} \times \mu_{2}-v_{1} v_{2}\right\|_{1} \leq\left\|\mu_{1}-v_{1}\right\|+\left\|\mu_{2}-v_{2}\right\| \leq\left\|\mu_{1}+\mu_{2}-v_{1} \pitchfork V_{2}\right\|$
$\left\|p_{r}-q_{n}\right\| \leq$
$\sum_{k}\left|p_{n, k}-q_{n, k}\right|$

$$
P_{n, k}^{k}=P\left(\sum_{k=1}^{1} \operatorname{Ber}\left(P_{n, k}\right)=m\right)
$$

| $\operatorname{Ber}\left(P_{n, 1}\right)$ | $\operatorname{Ber}\left(P_{n, m}\right)$ |
| :---: | :---: |
| $\mu_{1}$ | $\uparrow$ |

$M_{1} * M_{2} * M_{3} \cdots M_{2}$
u * â‹¯
Poisson (Pail =xpoisgon(Pn,m)
what is the I vertation setber

$$
\leq\left|1-p-e^{-p}\right|+\left|p-p e^{-p}\right|+P(\text { poissan }(p) \geqslant 2) 1-e^{-p}-p e^{-1}
$$

w/sh $e^{-p}-(1-p)$
![](https://cdn.mathpix.com/cropped/2025_11_26_bbc1444001dc06821efbg-5.jpg?height=156&width=342&top_left_y=1036&top_left_x=512)

$$
\begin{aligned}
& \angle e^{-p}-(1-p)+p-p e^{-p}+1-e^{-p}-p e^{-p} \\
& =2 p\left(1-e^{-p}\right) \leqslant 2 p^{2}
\end{aligned}
$$

