## Basics

(1) $P(A \triangle B) \leq P(A \triangle C)+P(C \triangle B)$
(2) if $P\left(A_{n} \Delta A\right) \xrightarrow[n \rightarrow \infty]{ } 0$ then $P\left(A_{r}\right) \rightarrow P(A)$ and $P\left(A_{r} \cap A\right) \rightarrow P(A)$
(3) if $P(A \cap \triangle A) \xrightarrow[n \rightarrow \infty]{ }$ o and $P\left(B_{n} \triangle A\right) \longrightarrow \infty 0$ then $P\left(A_{r} \cap B_{r}\right) \xrightarrow[n \rightarrow \infty]{ } P(A)$

$$
\begin{aligned}
& P\left(A_{n} \Delta A\right) \\
& \left(\begin{array}{rl}
= & P\left(A_{n}\right)-P\left(A_{n} \cap A\right) \\
& +P(A)-P\left(A_{n} \cap A\right) \\
& \vee P(A \cap \cap A) \rightarrow P(A) \\
P\left(A_{n}\right) & \rightarrow P(A)
\end{array}\right.
\end{aligned}
$$

$$
\begin{aligned}
& P\left(B_{n} \cap A\right) \rightarrow P(A) \\
& (1) \Rightarrow P\left(A_{n} \Delta B_{n}\right) \xrightarrow[n \rightarrow 00]{ } 0 \\
& P\left(A_{n}\right)-P\left(A_{n} \cap B_{n}\right) \rightarrow 0 \\
& P(A) \quad P(A)
\end{aligned}
$$

Hewitt-savage $\sigma-1$
Let $\left\{x_{k}\right\}_{k \geq 1}$ iid.
Let $A \in \sigma\left\{x_{k}\right\}_{k \geq 1}$ be penotatahe $(\pi A=A, \forall x$ - Finite permotatina)
Examble.

$$
P(A)=P(\pi A) \not \forall A \in \sigma\left\{x_{k}\right\}_{(\ll 1)}
$$

Consiver $A=\left\{\overline{\lim }_{n \rightarrow \infty} S_{n}>55\right\}$
Then $P(A)$ it $\{0,1\}$.
prof take $A \in G\left\{x_{k}\right\}_{k \geq 1}$
E Approofmate
$\exists A_{n} \in \sigma\left\{x_{1}, \ldots, x_{n}\right\}, n \geq 1$ so that $P\left(A_{n} \Delta A\right) \xrightarrow[n \rightarrow \infty]{ } 0$
So we know $P\left(A_{C}\right) \rightarrow P(A)$
Assure $A$ is permutable (from now on)
take a sey of $\{\pi\}_{n \geq 1}$ of finite permutator.
$\begin{aligned} P\left(A_{n} \Delta A\right)=P\left(\pi_{n}\left(A_{n} \Delta A\right)\right) & =P\left(\pi_{n}\left(A_{n}\right) \Delta A\right) \rightarrow 0 \\ & \searrow \\ I_{n}(A) & =A \\ \text { set qu. } & \end{aligned}$

$$
\begin{aligned}
& =P\left(r_{n}\left(A_{n}\right) \cap A_{n}\right) \rightarrow P(A) \\
& \left(\text { if } r_{n}\left(A_{n}\right), A_{n}\right. \text { are IND, } \\
& =P\left(r_{n}\left(A_{n}\right)\right) P\left(A_{i n}\right)=P^{2}\left(A_{n}\right) \rightarrow P^{2}(A) \\
& \text { Sog nos } \underbrace{n_{3}} r_{3}(4,5,6,12,3) \\
& (1,2,3,4,5) \rightarrow\left(x_{1}\right) \\
& A_{3} \in \sigma\left(x_{1}, x_{2}, t_{3}\right) \\
& r_{3}\left(A_{3}\right) \in \sigma\left(x_{4}, t_{5}, t_{6}\right)
\end{aligned}
$$

New chupter. : Corditioning. (Durnet ch. 5)

$$
\begin{aligned}
& \left(\Omega, \mathcal{F}_{0}, p\right) \quad \mathcal{F} \subset \mathcal{F}_{0} \\
& x \wedge x, E(X \mid)<\infty \\
& E(X \mid \mathcal{F}) \in E_{\mathcal{F}}(x) \\
& E_{\mathcal{F}}(f)=Y \Leftrightarrow 1 . Y \in \mathcal{F} \\
& \quad 2 . E\left(X^{\prime}, A\right)=E(Y, A), A \in \mathcal{Z}^{\prime} \\
& \quad(2) \Rightarrow(3) E(X \cdot Z)=E(Y \cdot z) \quad Z \in \mathcal{F} \text { and }|Z|<C_{\text {as }} .
\end{aligned}
$$

Exumples
Assume $E_{\mathcal{F}}(Z)=Y \quad E_{\mathcal{F}}(Z)=Y^{\prime}$ then $Y=Y$ as.
if not then $P\left(Y-Y^{\prime}>0\right)+P\left(Y-Y^{\prime}<0\right)$
create controdicton.
Assume wlog $p(\underbrace{y-y^{\prime}}_{A}>0)>0$

$$
\begin{gather*}
A \in \mathcal{F} \\
E[1 ; A]=E(X ; A)=E(Y ; A) \\
\Rightarrow E\left(Y-Y_{1} ; A\right)=0 \tag{$\rightarrow \curvearrowleft$}
\end{gather*}
$$

this ant huppor $P(A)>0$

Example (1) if $Z_{F}\left(\mathcal{F}_{\text {f }}\right.$ then $E_{F}(F)=\mathbb{E}$

Example (1) if $\underline{X} \in \mathcal{F}$ then $E_{\mathcal{F}}(\Psi)=\mathbb{R}$
(2) if $\{X, \mathcal{z}\}:$ in then $E_{f}(x)=E(x)$

Prove 2

$$
E(x \cdot z)=E(E(x) z, \quad \forall z \text { bdd } z \in z
$$

$\Omega \quad \widetilde{z}=\sigma\left\{A_{k}\right\} \begin{aligned} & E(X) E(z) \\ & \text { ston }\end{aligned}$

| $A_{2}$ | $A_{1}$ | $A_{3}$ |
| :--- | :--- | :--- | :--- |
| $A_{4}$ | $A_{5}$ | $A_{6}$ |

$E(X)\left(=\frac{E\left(K: A_{12}\right)}{P\left(A_{2}\right)}\right.$ if $w \in A_{k} \quad k=I_{1 . \cdots}$ The purpose of fausformotion
for
![](https://cdn.mathpix.com/cropped/2025_11_25_72b5e6707690a11f91bfg-3.jpg?height=516&width=522&top_left_y=704&top_left_x=1256)

Rador - nikodym.
$\left(\Omega, \mathcal{I}_{0}\right)$ measiore space.
$\mu \ll P$ ( $\mu$ is Absolutely condroos wrat, $P$ )
$Q \sim$ signifinite mearuce
if $A \in \mathcal{F}_{0}$ and $P(A)=0$ then $M(A)=0$
Ex let $\delta_{x, y}(x, y)$ is joint density of $(x, y) \in \mathbb{R}^{2}$
then $\begin{gathered}E(Y) \\ \sigma\left\{x^{\prime}\right\}\end{gathered}=\int_{-100}^{\infty} y \delta_{y \mid Z=0}(x ; y) d y$

$$
f_{Y \mid X=x_{0}}\left(x_{0}, y\right)=\frac{f_{X Y}\left(x_{0}, y\right)}{f_{X}\left(x_{0}\right)} \quad f_{X}\left(x_{0}\right)=\int_{-\infty}^{\infty} f\left(x_{0}, y\right) d y
$$

