LP. P71 Doob's inequarity
Let $\left\{x_{n}, y_{s}\right)_{n \geq 0}$ be submg ( $x_{n} \geq 0$ a.s. $n \geq 0$ )
Then $E\left(\max _{0 \leqslant k \leqslant n}\left(x_{k}\right)^{p}\right) \leq E\left(x_{n}^{p}\right)\left(\frac{p}{1-p}\right)^{p} \quad p=2=\left(\frac{p}{p-1}\right)^{p}=4$.
Remark: For submg. which ist positive use $\left(X_{n}^{+}, F_{n}\right)_{n>0}$
For Reg mg. "" ".. " " $\left(\left|X_{n}\right|, \widetilde{F}_{n}\right)_{n>0}$
Application: (et $\left\{x_{n} f_{n}\right\}_{n \geq 0}$ be $M G$ and $\sup _{n \geq 0} E\left(\left|x_{n}\right|^{p}\right)<\infty$ then (1) $x_{n} \xrightarrow[n \rightarrow \infty]{\text { a. } 5 .} x$
(2) $E\left[\mid x_{n}^{n-\infty} x^{p}\right] \xrightarrow[n \rightarrow \infty]{ } 0$ By $\operatorname{Det}$.
why? $\left|x_{n}-x\right|^{p} \leq 2^{p} \max _{1 \leq k \leq n}\left|x_{n}\right|^{p}$
Since $x_{n}, x$ is two, $2^{p}$. and the use the Biggent $t_{n} 1 \leq k \leq n$ Dominating function
If we wart $E\left|x_{n}-x\right|$ we have $\sup _{n \geq 0} E\left(\left|x_{n}\right|^{p}\right)<\infty \Rightarrow$ uniform ingrebility. then $E\left(x_{n}-x\right)=0$.
Application for $P=2$. Branching. Processes. $\left\{\xi_{n}\right\},\left\{\xi_{n, i}\right\}_{i \geq 0, n>0}$ I wd. 2 ... $\forall n\left\{\xi_{n}, i\right\}_{i>1}$ iid. Libe \# of children of Eah indidual

$$
P(\xi=0)>0 \quad M=E(\xi)=\sum_{k=0}^{\infty} k P(\xi=k)<\infty
$$

$z_{n+1}=\sum_{k=1}^{Z_{n}} \xi_{n+1} \cdot i \quad z_{n}=\#$ of People in the $n^{+L}$ Generators.
$y_{n}=\sigma\left\{z_{1}, \ldots, z_{n}\right\}_{n \geq 1}$
$\operatorname{daim}\left(\frac{Z_{n}}{\mu r}, \mathcal{F}_{n}\right\}_{1 \geq 0} \mu G$.
cook At $E_{z_{n}}\left(\frac{Z_{n+1}}{\mu^{n+1}}\right)=\frac{\mu \cdot Z_{n}}{\mu^{n+1}}=\frac{Z_{n}}{\mu_{n}}$
this Euest is Extinction. integers converge iff Betomes Constent.

Result if $\mu \leq 1$ then $Z_{n} \xrightarrow[n \rightarrow \infty]{0.5 .} 0 \quad \begin{aligned} & \text { Integers Converge } \\ & \text { Betomes Constant }\end{aligned}$
$\exists T$ aoo with $Z_{T}=0$ : Extincter.
$e=P($ Extinction $)$ or $e=1$
Proof: $\quad Z_{n}=\underbrace{Z_{n}}_{\mu n} \underbrace{\mu^{n}}$
. H monotone

Proof: $\quad Z_{n}=\frac{t_{n}}{\mu_{n}^{r}} \underbrace{\mu^{n}}$
MG monotone
non Increasing.
$M \leq 1 \Rightarrow\left\{z_{r}, \mathcal{F}_{n}\right\}_{n \geq 0}$ is super $M 6, z_{n}>0 \forall_{n}$
â‡’ By MGCT $\Rightarrow Z_{n} \xrightarrow[n \rightarrow \infty]{\text { a.s. }} Z_{00} \equiv 0$
(2). F $\mu>1$ then $e<1$

How solve w/o Poob. LPinequality
Sketch proof of (2)
Prob. Generating function New concrept.
$\varphi(\xi)(s)=E\left(s^{\xi}\right)=\sum_{k=0}^{\infty} P(\xi=k) \cdot \delta^{k}, \quad 0 \leq s \leq 1$
increasing '3. Convex
it follows $e=\varphi\left(e^{\xi}\right)=\sum_{k=0}^{\infty} P(\xi=k) e^{k}$
$\varphi^{\prime} \geq 0 \quad \varphi^{\prime \prime} \geq 0$

NEED solution for

$$
\begin{aligned}
& \varphi(\xi)(1)=1 \\
& \varphi(\xi)(0)=P(\xi=0)>0
\end{aligned}
$$

![](https://cdn.mathpix.com/cropped/2025_11_25_a187e21cca6570fd093fg-2.jpg?height=314&width=565&top_left_y=1205&top_left_x=354)
$P(3=0)=$

Now we use Doob (in the context of $\mu>1$ )
(1) iff $\operatorname{Var}\left[y^{2} y^{2}\right]=\sigma^{2}<\infty, \quad \mu>1, \quad P(z=0)>0$
$0 \leqslant X_{n}=\frac{Z_{n}}{\mu^{n}} n \geq 0$ is $m g$. We get $X_{n} \xrightarrow[\Lambda \rightarrow \infty]{\text { a.s. }} X$
$E_{Z_{n-1}}\left[\left(X_{n}-X_{n-1}\right)^{2}\right]$ like the conditional uarionce.
$D_{n}$ - the martingate D. Eference.

$$
=E_{f_{n-1}}\left(\frac{z_{n}}{\mu^{n}}-\frac{z_{n-1}}{\mu^{n-1}}\right)^{2}=\mu^{-2 n} E\left[z_{n}-\mu z_{n-1}\right]^{2}
$$

take $\mu^{2 n}$ out. and leame one $\mu$

$$
\begin{array}{ll}
z_{n}=\sum_{i=1}^{z_{n-1} \xi_{n, 1}} & =\mu^{-2 n} \sigma^{2} \cdot z_{n-1} \\
E\left(z_{n-1}\right)=\mu^{n-1} k \\
E\left(x_{n}-x_{n-1}\right)^{2}=\mu^{-2 n} \sigma^{2} \mu^{n-1}=\mu^{-(n+1)} \sigma^{2}
\end{array}
$$

$$
\begin{aligned}
& E\left(X_{n}^{2}\right)= \\
& X_{n}^{2}=\left[1+\sum_{k=1}^{n}\left(X_{k}-X_{k-1}\right)\right]^{2} \Rightarrow E\left(X_{n}^{2}\right)=1+\sigma^{2} \sum_{k=1}^{n} m^{-(k+1)}
\end{aligned}
$$

$\left\{D_{k}\right\}_{k=1} M D$.
$E\left(D_{k} D_{m}\right)=0 \mathrm{kkm}, E\left(D_{k}\right)=0$.

$$
\operatorname{Sup}_{n \geq 0} E\left(X_{n}^{2}\right) \leq 1+\sigma^{2} \sum_{k=1}^{\infty} \mu^{-(k-1)}<\infty
$$

if this is finite $B_{y} L^{p} d$ ood Inequelty
we get $E\left(x_{n}-x\right)^{2} \xrightarrow[n \rightarrow \infty]{ } 0 \Rightarrow E\left|x_{n}-x\right| \xrightarrow[n \rightarrow \infty]{ } 0 \Rightarrow E(x)=1$ vote (1) $\uparrow$ kesten-stigure
Optimal Result: Assume $\mu>1, \frac{z_{n}}{m} \xrightarrow{\text { A.s. }} 0$ w.P. 1
iff

$$
E\left(\xi \cdot \operatorname{cog}^{+}(\xi)\right)<\infty
$$

