$\left\{\bar{x}_{n}, \tilde{\sigma}_{n}\right\}_{0 \leq n \leq N}$ somm. $\quad$ (Durrett 55.7 P. 229 )
$T$ stopping time(s.t.) $0 \leq T \leq N$
ve saw $E\left(X_{0}\right) \leq E\left(X_{i}\right) \leq E\left(X_{\pi}\right)$

$$
D_{k}=X_{k}-X_{k-1} \quad(H \cdot X)_{n}=\sum_{k=0}^{n} H_{k} \cdot D_{k} \quad H_{n} \in \mathcal{F}_{n-1}
$$

Easy wey tuke $H=1 H_{K} \geq 0 \Rightarrow\left((H \cdot x)_{N}, \mathcal{F}_{N}\right)$ submb.

$$
\begin{aligned}
& (H \cdot x)_{N}=X_{T} \cdot X_{0} \\
& E(H \cdot x)_{0}=0 \quad H_{k}=1_{\xi \leqslant} \geq 0
\end{aligned}
$$

(2) Take $S$ s.t. $S \leq T$ ans. $(0 \leq S \leq T \leq N)$
then $E\left(X_{S}\right) \leq E\left(X_{T}\right)$

$$
\begin{aligned}
y_{n} & =X_{T \wedge n} \quad 0 \leq n \leq N \quad\left\{Y_{n}, Y_{n}\right\}_{0 \leq n \leq N} \text { submg. } \\
E\left(Y_{0}\right) & \leq E\left(Y_{s}\right) \leq E\left(Y_{N}\right) \\
E\left(X_{0}\right) & \leq E\left(X_{s}\right) \leq E\left(X_{T}\right) \leq E\left(X_{N}\right)
\end{aligned}
$$

(3) $S \leq T$ both S.T. $\left\{X_{n}, F_{n}\right\}_{0 \leq n \leq N}$ Subme.

$$
\begin{aligned}
& E\left(X_{T}\right) \geq X_{S} \\
& E\left(X_{T} ; A\right) \geq E\left(X_{S} ; A\right) \quad \forall \in \tilde{F}_{S} .
\end{aligned}
$$

Define $\tilde{S}=\left\{\begin{array}{ll}S & \text { on } A \\ T & \text { on } A^{c}\end{array} \quad \tilde{S} \leq T\right.$

$$
E\left(x_{5}\right) \leq E\left(x_{T}\right)
$$

Dear. $E\left(x_{5} j A^{c}\right)=E\left(x_{T} ; A^{c}\right)$
we get

$$
\begin{aligned}
& E\left(X_{s} ; A^{c}\right) \leq E\left(X_{T} ; A\right)=E\left(E_{\tilde{\partial s}_{s}}\left(X_{T}\right) ; A\right), \quad A \in \tilde{f r}_{s} \\
& \therefore \Rightarrow \quad X_{s} \leq E_{\tilde{\partial}_{s}}\left(X_{T}\right) \text { as. }
\end{aligned}
$$

Now $N=\infty$.
Two methods. 1. show $X_{s} \leq 1=\mid 2 E_{z_{s}}\left(X_{T}\right)$ a.s.

1) LI method. works for ${ }^{1}$ MG, sub, sup.
2) Using Fatur Lemma wonks for Position sop MG.

Theoren let $\left\{x_{n}, F_{n}\right\}_{n \geq 0}$ UI, sub MGn
then if $T$ is S.T ( $\{T=\infty\}$ maybe nontrival)
then $\left\{X_{T \wedge n}, F_{n}\right\}_{n \geq 0}$ is $L I$ as well
Proof: since $\left\{X_{n}\right\}_{n z 1}$ is LII then ne nect work $X_{n} \xrightarrow[n \rightarrow \infty]{\text { as. } L^{\prime}} X_{\infty}$ convex, nondecreesiany. Then $\left\{X_{n}^{+}, \tilde{\mathscr{Z}}_{n}\right\}_{n \geq 0}$ sob $M G$. So, $E\left(X_{T \wedge n}^{+}\right) \leq E\left(X_{n}^{+}\right)$all positive.

$$
\Rightarrow \sup _{n \geq 0}\left\{\left(X_{T_{n n}}^{+}\right)\right\} \leq \sup _{n \geq 0}\left\{E\left(X_{n}^{+}\right)\right\}<\infty \quad \begin{aligned}
& \text { Confition for } \\
& \text { Courergen of } \\
& \text { Mf Eg. The Thearm. }
\end{aligned}
$$

we get by MGCT
(1) $X_{T \cap n} \xrightarrow[n \rightarrow \infty]{\text { a.s. }} X_{T}$
(2) $E\left(\left|x_{T}\right|\right)<\infty \quad \infty$
$\left|x_{\text {TNN }}\right| \leqslant\left|x_{T}\right|+\left|x_{n}\right|$ as.
we hure seen
$\left\{x_{\alpha}\right\}_{\alpha \in A} \quad\left\{Y_{\beta}\right\}_{\beta \in B}$ are both UI
ther $\left\{X_{\alpha}+X_{\beta}\right\} \alpha \in A, \beta \in B$ is $U I$ as well.
(1) theosen 2 Let $\left\{x_{n}, y_{n}\right\}_{n \geq 0}$ LI sub. subs let $0 \leq T \leq 0$ be ș).
then $E\left(x_{0}\right) \leqslant E\left(x_{T}\right) \leqslant E\left(x_{\infty}\right)$
Proof $\quad \forall 0 \leq n \leq \infty$
![](https://cdn.mathpix.com/cropped/2025_11_25_37814a0d5382cfe47037g-2.jpg?height=235&width=1347&top_left_y=1650&top_left_x=318)

Corollarg.
(2) : $S \leq t ~ S-S_{A}$
then $E\left(X_{S}\right) \leqslant E\left(X_{T}\right)$
(3) $x_{S} \leq \underset{y_{n}}{E}\left(x_{T}\right)$, an.

Simple Rerriom walk Not Symmetric.
Ex simple Rendom walk which is not symuetric
$\left\}_{k k}\right\}_{k \geq i} i i d \quad\left\{\frac{p}{q}-1_{+1}^{-1}\right.$ where $p>q \quad p+q=1 \quad \begin{array}{l}1 \geq p>1 / c \\ 0 \leq q<1 / k\end{array}$

$$
S_{n}=\sum_{k=1}^{n} \xi_{k}, n \leqslant 0 \quad S_{0} \equiv 8 \quad 0 \leq 9<k
$$

Let $x \in \mathbb{Z} \quad T_{x} \equiv \inf \left\{n i S_{n}=x\right\}$.
if $b>0$, then $T_{b}<\infty$ as.

$$
\begin{aligned}
& \frac{S_{n}}{n} \underbrace{\text { as. }}_{n \rightarrow \infty} E(\xi)=p-q>0 . \\
\Rightarrow & S_{n} \underset{n \rightarrow \infty}{a .4 .5} \infty
\end{aligned}
$$

$$
\frac{q}{p}<1 \Rightarrow\left(\frac{q}{p}\right)^{x}<1
$$

Claim: $a<0<b$.
then $p\left(T_{a}<T_{b}\right)=\frac{\varphi(b)-\varphi(0)}{\varphi(b)-\varphi(a)} \quad \varphi(x)=\left(\frac{q}{p}\right)^{x}, x \in \mathcal{Z}$
(1) $\left\{\left\{\varphi\left(\delta_{n}\right), \mathcal{F}_{n}\right\}_{n \geq 0}\right.$ is a $\mu_{g}$ ?

$$
\begin{aligned}
E_{F_{n}}\left(\varphi\left(s_{n+1}\right)\right) & =E_{F_{n}}\left[\left(\frac{q}{p}\right)^{\alpha}\right. \\
& =E_{F_{n}}\left[\left(\frac{q}{p}\right)^{s_{n}} \cdot E\left(\frac{q}{p}\right)^{3 n+1}\right. \\
& =\left(\frac{q}{p}\right)^{5 n} \cdot E_{F_{n}}\left(\frac{q}{p}\right)^{3 n+1} \text { whech } \xi_{n+1} L_{F_{n}} \\
& =\left(\frac{q}{p}\right) p+\left(\frac{q r}{p}\right)^{1} \cdot q \\
& =q+p=1
\end{aligned}
$$

Defe $T=T_{a} \wedge T_{b},<\infty$ as.

$$
\begin{gathered}
\left\{\varphi\left(S_{T M 1}\right), F_{n}\right\}_{n 20} \text { is } 11 G . \\
0 \leq \varphi\left(S_{T M n}\right) \leq\left(\frac{q}{P}\right)^{a}=\left(\frac{P}{q}\right)^{-a}
\end{gathered}
$$

(ii) $\varphi\left(S_{T A n}\right) \leqslant\left(\frac{P}{a}\right)^{-a}$, nzo. sheas Bourded. ∴ LII
$\Rightarrow\left\{\varphi\left(S_{T \wedge n}\right)\right\}_{n z o} \Delta I$
we got by on results.

$$
\begin{aligned}
& E\left(\varphi\left(S_{+}\right)\right)=E\left(\varphi\left(S_{0}\right)\right)=1 \\
& S_{T} \in\{a, b\} \\
& E \varphi\left(S_{T}\right)=P\left(T_{a}<T_{b}\right) \cdot\left(\frac{a}{P}\right)^{a}+P\left(T_{b}<T_{a}\right)\left(\frac{q}{P}\right)^{b} \\
& P\left(T_{a}<T_{0}\right)+P\left(T_{b}<T_{a}\right)=1
\end{aligned}
$$

Two equation two unknowns solve and get

$$
\begin{aligned}
& P\left(T_{a}<T_{b}\right)=\frac{\varphi(b)-\varphi(0)}{\varphi(b)-\varphi(a)} \xrightarrow[b \rightarrow 00]{ } \frac{0-1}{0-\left(\frac{a}{p}\right)^{a}}=\left(\frac{p}{a}\right)^{a} . \\
& E\left(T_{b}\right)
\end{aligned}
$$

