$M G$ For $B M . \quad(\Omega, \mathcal{F}, P)$
Def. of MG in continuous time
$\left\{X_{t} \mathcal{J}_{t}\right\}_{t \geq 0}$ is $M t$ if (1) $E\left|X_{t}\right|<\infty$
(2) $x_{t} \in y_{t}$
(3) $E_{f_{t}}\left(X_{t+h}\right)=X_{t} \quad \forall t \geq 0, h>0$
we want to study MG Associated with BM.
$M(x, t), x \in \mathbb{R}, t \geq 0$ wl vatural filtation $\left.\left\{\mathcal{F}_{t}\right\}\right\}_{t \geq 0}$ or conarical fitration. $M(x, t) \quad x \in \mathbb{R}, t \geq 0$.
Question when is $\left\{\mu\left(B_{t}^{x}, t\right), \mathcal{F}_{t}\right\}_{t 20}$ a $\mu G$ ?

$$
E_{x} \mu\left(B_{t+h}, t+h \mid f_{t}\right)=M\left(B_{t}^{x}, t\right) \text { a.s. } \forall_{x} \in \mathbb{R}, t>0, h>0
$$

![](https://cdn.mathpix.com/cropped/2025_11_25_45ad7a108baa9e929d14g-1.jpg?height=263&width=1271&top_left_y=1514&top_left_x=192)
$\varphi(y)=E_{y}\left[\mu\left(B_{n}, t+h\right)\right]$

Example Famous MGExonential

$$
\begin{array}{ll}
\mu(x, t)=e^{\theta x-\theta^{2} \frac{t}{2}} \quad \theta \in \mathbb{R}, \theta \text { constant. } & \\
E_{x}\left(\mu\left(B_{n}, t+h\right)\right)=E_{x}\left(e^{\theta B_{n}-\theta^{2}(t+h) / 2}\right) & B_{n} \sim N(x, h) \\
=e^{-\theta^{2}(t+h) / 2} \cdot E_{x}\left(e^{\theta B_{n}}\right) & B_{n} \stackrel{\theta}{=} x+\sqrt{h} E \sim N(0,1) \\
=e^{-\theta^{2}(t+h) / 2}, \ldots, E^{\theta(x+\sqrt{h} z)} &
\end{array}
$$

$$
\begin{aligned}
= & e^{-\frac{\theta^{2}(t+h) / 2}{2}} \\
e^{-\frac{\theta^{2} t}{2}} e^{-\frac{\theta^{2}}{2}} & \underbrace{E\left(e^{\theta x} e^{\theta(x+\sqrt{h} z)} k_{2}\right.} \\
e^{-\frac{\theta^{2} t}{2}}+\theta x & =\mu(x, t)
\end{aligned}
$$

$\left(e^{\theta B_{t}^{4}-\frac{\theta^{2} t}{2}}, \widetilde{d_{t}}\right)_{t \geq 0}$ is $m g$ wnt. $P_{x} x \in \mathbb{R}$
$\partial \theta$

$$
\begin{aligned}
& E_{x}\left[\mu\left(B_{n}, t+h ; \theta\right)\right]=\mu(x ; t ; \theta)_{\gamma\{\theta \theta} \\
& E_{x}\left[\frac{\partial}{\partial \theta} \mu\left(B_{n}+t+h ; \theta\right)\right] \quad \frac{\partial}{\partial \theta} \mu(x, t, \theta) \quad \forall \theta \\
& \left\{\mu \left(B_{t}^{x}\left(, \theta, \tilde{f}_{t}\right\} \text { is } \mu g .\right.\right. \\
& \left.\partial_{\partial \theta}^{\mu}\left(B_{t}^{+}, t, \theta\right), \tilde{f}_{t}\right\} \quad \mu_{t} .
\end{aligned}
$$

Continue to take Derivetives $\frac{\partial^{2}}{\partial \theta^{2}} \cdot \mu(k) \forall \theta$

$$
\begin{aligned}
& \mu(\cdot)=e^{\theta x-\theta^{2} t / 2} \\
& \frac{\partial}{\partial x} \mu(\cdot)=\mu(\cdot)(x-\theta t) \\
& \theta=0 \\
& \left.\Rightarrow \frac{\partial}{\partial \theta} \mu(0)\right|_{\theta=0}=x \\
& \Rightarrow\left\{B_{t}^{x}, \tilde{F}_{t}\right\}_{t \geq 0}
\end{aligned}
$$

Eundies Brownown motow is my.

$$
\begin{aligned}
& \frac{\partial^{2}}{\partial \theta^{2}}=\left.\mu() \cdot(x-\theta t)^{2}\right|_{\theta=0 .}=x^{2} \\
& \Rightarrow\left(B_{t}^{2}-t F_{t}\right)_{t \geq 0} \\
& \frac{\partial^{3}}{\partial \theta^{3}}=\mu()(x-\theta t)^{3}+\mu() 2(x-\theta t)(-t)-t \mu(0)(x-\theta t) \\
& \left.\Rightarrow B_{t}^{3}-3 t B_{t}, F_{t \rightarrow 0}\right\} M_{6} . \\
& \theta=0
\end{aligned}
$$

Mr. that we get: $1, B_{t}, B_{t}^{2}-t, B_{t}^{3}-3 t B_{t}, B_{t}^{4}-6 t B_{t}^{2}+3 t^{2} \ldots$

In the Book Let $\mu(x, t)$ satify $\frac{\partial \mu}{\partial t}+\frac{1}{2} \frac{\partial^{2} \mu}{\partial t^{2}}=0 \quad \forall_{x} \in R, t>0$
then $M\left(B_{t}, t\right)$ is $M f$.
the Book Proved $\frac{\partial}{\partial t} E_{x}\left(M\left(B_{t}, t\right)\right)=0$
$\Leftrightarrow \quad E_{x} M\left(B_{t}, t\right)=M(x, 0) \forall t \geq 0, x \in \mathbb{R}$.
Stentints.

$$
P_{t}(x, y)=P_{N(x, t)}(y),+ \text { torss out } \quad \frac{\partial P_{t}}{\partial t}=1 / 2 \frac{\partial^{2} P_{t}}{\partial y^{2}} \quad \forall x \in \mathbb{R} \text {. }
$$

r s.t. $\quad \tau \leq t$ as. $\quad E_{\mathcal{F}}\left(M\left(B_{t}, t\right)\right)=M\left(B_{\phi}, \delta^{\top}\right)^{\top}$

