![](https://cdn.mathpix.com/cropped/2025_11_25_6588446aaf845e338ac5g-1.jpg?height=128&width=426&top_left_y=292&top_left_x=253)

$$
T=T_{b} \wedge T_{a} .
$$

$$
\begin{aligned}
& \text { Question } P_{0}\left(T=T_{a}\right)=P_{0}\left(T_{a}<T_{b}\right) \\
& \left|B_{T \wedge t}\right| \leq b \vee|a| \quad \forall t \geq 0 \Rightarrow U I \\
& B_{T \wedge t} \underset{t \rightarrow \infty}{\text { a.s. }} B_{T} \\
& E_{0}\left[B_{T \wedge t}\right]=E_{0}\left(B_{0}\right)=0 \\
& \text { DCT } \downarrow t \rightarrow \infty \\
& E_{0}\left(B_{t}\right)=0=P\left(T_{a}<T_{b}\right) \cdot a+P\left(T_{b}<T_{a}\right) b . \\
& P\left(T_{a}<T_{b}\right)+P\left(T_{a}>T_{b}\right)=1 \\
& B_{T_{a}}=a \\
& B_{T_{b}}=b \\
& \Rightarrow P\left(T_{a}<T_{b}\right)=\frac{b}{b-a}=\frac{b}{b+|a|} \\
& P\left(T_{b}<T_{a}\right)=\frac{|a|}{b+|a|}
\end{aligned}
$$

![](https://cdn.mathpix.com/cropped/2025_11_25_6588446aaf845e338ac5g-1.jpg?height=246&width=458&top_left_y=1746&top_left_x=281)
translate to the zero case

$$
\left.\begin{gathered}
b-x \\
0 \\
a-x
\end{gathered} \right\rvert\, \sim \cdots \cdots \cdots
$$

$\Delta I \Rightarrow E\left(M_{i}\right) \underset{t \rightarrow \infty}{\rightarrow} D$
![](https://cdn.mathpix.com/cropped/2025_11_25_6588446aaf845e338ac5g-3.jpg?height=367&width=1268&top_left_y=228&top_left_x=265)
if $\frac{B_{t}}{t} \xrightarrow[t \rightarrow \infty]{\text { ans. }} 0$ then $B\left(\frac{1}{t}\right) \xrightarrow[t \rightarrow \infty]{ } Y \equiv 0$

$$
B(0)=0
$$

$$
\begin{aligned}
& E\left(e^{\theta \cdot B_{t \wedge T}-\frac{\theta^{2}}{2}(T \wedge t)}\right]=1 \quad \forall t>0 \\
& B_{t \wedge T} \leq a+b(t \wedge T), t \geq 0 \\
& \theta=2 b \\
& E\left(e^{2 b B_{t \wedge T}-2 b^{2}(T \wedge t)}\right] \\
& \leq e^{2 b[a+b(t \wedge T)]-2 b^{2}(T \wedge t)} \\
& \leq e^{2 a b}
\end{aligned}
$$

$$
\begin{aligned}
& \mu(t \cap T) \leq e^{2 a b}, \quad \begin{array}{l}
t \geq 0 \quad a \cdot \swarrow^{a b T} \\
E_{0}[M(t \wedge T)] \underset{t \rightarrow \infty}{a . s}\left\{\begin{array}{l}
M_{T}=e^{2 b B_{T}-2 b^{T} T} \text { if }\{T<\infty\} \\
=e^{2 a b .} \\
M_{T}=0 \quad \text { on }\{T=\infty\}
\end{array}\right.
\end{array} \text { }
\end{aligned}
$$

we show since SLLN argurent

$$
\begin{gathered}
E_{0}\left(M_{T}\right)=E_{0}\left[e^{2 a b} j T<\infty\right)=1 \\
0 \cdot P(T=\infty) \\
P_{0}(T<\infty)=e^{-2 a b}
\end{gathered}
$$

$\underline{E}_{x}$ R.V. $X$

| $x$ | $-7 / 4$ | 1 | 2 |  |
| :---: | :---: | :---: | :---: | :---: |
| $p(x)$ | -4 | .5 | .1 | $=1$ |

Define a stopping time $\tau$ such ThuT $B_{\tau}^{0} \stackrel{g}{=} x$

$$
\begin{gathered}
\tilde{f}_{1}=\sigma\{x=-7 / 4, x \in\{1,2\}\} \\
\text { wth. } E_{f_{1}}(x)= \begin{cases}-7 / 4 & : x=-7 / 6 \\
x_{1} & \frac{1.5+2.1}{6} x \in\{1,2) \\
\leq 7 / 6\end{cases}
\end{gathered}
$$

$$
\begin{aligned}
& E\left(x_{1}\right)=0 \\
& B_{r_{1}} \stackrel{D}{=} x_{1} \\
& \tau_{1}=T_{7 / 6} \wedge T_{-7 / 4}
\end{aligned}
$$

